theories/KnapsackCode2.v
@@ -1,0 +1,16 @@
+From stdpp Require Import numbers list.
+From CoqCP Require Import Options Imperative Knapsack KnapsackCode.
+From Generated Require Import Knapsack.
+From Coq Require Import ssreflect ssrfun ssrbool.
+Set Implicit Arguments.
+Unset Strict Implicit.
+Unset Printing Implicit Defensive.
+
+Lemma extractAnswerEq (items : list (nat * nat)) (limit : nat) (hp : ((limit + 1%nat) * (length items + 1%nat) <= 1000000%nat)%nat) (a32 : forall x, (fst (nth x items (0%nat,0%nat)) < 2^32)%nat) (b32 : forall x, (snd (nth x items (0%nat,0%nat)) < 2^32)%nat) : extractAnswer (start items limit) = Z.of_nat (knapsack items limit).
+Proof.
+  unfold start, invokeContract, state at 1. case_decide as uu; [| easy].
+  fold state.
+  unfold funcdef_0__main at 2. unfold getCommunicationSize.
+  rewrite pushDispatch2 unfoldInvoke_S_GetCommunicationSize dataLength pushNumberSet.
+  rewrite pushNumberGet2.
+Admitted.
